\begin{proposition}
  Let 
  $f : \R^n \to \R$ 
  be continuous such that 
  a minimum $x^*$ exists and is unique.
  Then 
  for all $y \in \R^n$ and $C>0$ 
  it follows
    \begin{gather}
      \inf_{\norm{\Delta}=C} f(y+\Delta) - f(y) > 0 \qquad
      \Rightarrow \qquad 
      \norm{x^* - y} \le C.
    \end{gather}
\end{proposition}


\begin{proof}
Since 
$\mathcal{C}:=\left\{ \norm{\Delta}\le C \right\}$
is compact and
\begin{gather*}
  f(x^*) \le f(y) <  \inf_{\norm{\Delta}=C} f(y+\Delta)
\end{gather*}
the continious function $f(y+\,\cdot\,)$ has a minimum in 
$\overset{\circ}{\mathcal{C}}:=\left\{ \norm{\Delta} < C \right\}$. 
Since 
$x^*$ is the unique minimum of $f$
there exists $\Delta^* \in \overset{\circ}{\mathcal{C}}$ 
such that 
$x^* - y = \Delta^*$.
We conclude that
$\norm{x^* - y} \le C$.
\end{proof}

 %%%%%%%%%%%%%%%%%%%%%%%%%%%%%%%%%%%%%%%%%%%%%%%%%%%%%%%%%%%%%%%%

\begin{proposition}
  Let 
  $f\in C^2(\R)$. 
  Then
  for all $a,x,\Delta \in \R^n$ 
  there exist $\xi_1, \xi_2 \in (0,1)$ 
  such that it holds
  \begin{gather}
    \label{syu_2.result}
    f(a^T (x + \Delta)) - f(a^T x) = 
    f^{'}(a^T x)\, \Delta^T a + 
    \xi_1 f^{''}(a^T (x + \xi_1\xi_2 \Delta))\, \Delta^T A\ \Delta,
  \end{gather}
  where 
  $A:= a a^T \in \R^{n \times n}$ .
\end{proposition}

\begin{proof}
  By the chain rule 
  we have
  for all $a, x, \Delta \in \R^n$ and $\xi \in (0,1)$
  \begin{gather}
    \label{syu_2.0}
    \nabla_x f(a^T (x + \xi \Delta)) =
    f^{'}(a^T (x + \xi \Delta))\, a.
  \end{gather}
  By 
  the mean value theorem and \eqref{syu_2.0}
  there exist $\xi_1, \xi_2 \in (0,1)$
  such that
  \begin{align}
    \label{syu_2.1}
    \begin{split}
    f(a^T (x + \Delta)) - f(a^T x)
    &= 
    \Delta^T\, \nabla_x f(a^T (x + \xi_1 \Delta)) \\ 
    &=
    f^{'}(a^T (x + \xi_1 \Delta))\, \Delta^T a.
    \end{split}
  \end{align}
  and
  \begin{gather}
    \label{syu_2.2}
    f^{'}(a^T (x + \xi_1 \Delta)) - f^{'}(a^T x)
    =
    \xi_1 f^{''}(a^T (x + \xi_1 \xi_2 \Delta))\, a^T \Delta.
  \end{gather}
  Plugging \eqref{syu_2.2} in \eqref{syu_2.1} 
  yields
  \eqref{syu_2.result}.
\end{proof}

