\begin{theorem}
  The estimate 
  \begin{gather}
    \sqrt{N}
    \left( 
  \frac{1}{N}
    \sum_{i=1}^{n} 
    w_i
    \mathbf{1}
    _{\left\{ Y_i\le t \right\}}
    -
    \P[Y(1)\le t]
    \right)
  \end{gather}
  is Asymptoticaly normal.
\end{theorem}
\begin{proof}
The term 
\begin{gather}
    \left|  
  \frac{1}{N}
    \sum_{i=1}^{N} 
    \left( 
    T_i
    w_i
    -
    1
    \right)
    \left( 
    \P[Y(1)\le t | X_i]
    -
    \inner
    {B(X_i))}
    {\lambda^*}
    \right)
  \right|
\end{gather}
gives back the expectation. We control its rate 
with the factor of basis rates and primal weights.
Choose $d$ to be faster than $\sqrt{n}$.
The rest follows with standard empirical theory.
Expectations are 0.
$\norm{\delta}$ has to converge fast enough.
\begin{align*}
  &
  \sqrt{N}
  \cdot
  \E
  \left[ 
    \left( 
    T
    \cdot
    w(X)
    -
    1
    \right)
    \left( 
      \P
      [
      Y(1)\le t
      |X
      ]
      -
      \inner
      {B(X)}
      {\lambda^*}
    \right)
  \right]
  \\
  &
  \ 
  =
  \ 
  \sqrt{N}
  \cdot
  \E
  \left[ 
    \pi(X)
    \cdot
    \left( 
    w(X)
    -
    1
    /
    \pi(X)
    \right)
    \left( 
      \P
      [
      Y(1)\le t
      |X
      ]
      -
      \inner
      {B(X)}
      {\lambda^*}
    \right)
  \right]
  \\
  &
  \ 
  \le
  \ 
  \sqrt{N}
  \cdot
  \E
  \left[ 
    \left| 
    w(X)
    -
    1
    /
    \pi(X)
    \right|
    ^2
    \right]
    ^{1/2}
  \E
  \left[ 
    \left| 
      \P
      [
      Y(1)\le t
      |X
      ]
      -
      \inner
      {B(X)}
      {\lambda^*}
    \right|
    ^2
    \right]
    ^{1/2}
    \\
  &
  \ 
  \le
  \ 
  C
  \sqrt{N}
  \sqrt{\log(N)}
  N^{-1/(d+2)}
  \cdot
  N^{-1/(d+2)}
    \\
  &
  \ 
  \le
  \ 
  C
  \sqrt{\log(N)}
  N^{-1/6}
  \to 0
  \qquad
  \text{for}\ 
  N\to\infty
\end{align*}
Note, that we get no convergence for $d>1$. 
Also note that
\begin{gather*}
  \E
  \left[ 
    T
    \cdot
    w(X)
    -
    1
    |
    X,
    X_1,
    \ldots,
    X_N
    \right]
    =
  \E
  \left[ 
    T
    |
    X
    \right]
    w(X)
    -
    1
    =
    \pi(X)
    \left( 
      w(X)
      -
      1/\pi(X)
    \right)
\end{gather*}
\end{proof}
