 \begin{align*}
   \left| 
   1 / \pi_i
   -
   w_i
   \right|
   & 
   \ 
   =
   \ 
   \left| 
   1 / \pi_i
   -
   (
      f ^ { ' }
   )
   ^ {-1}
   \left( 
   \inner
   { B(X_i)}
   { \lambda ^ \dagger }
   +
   \lambda^\dagger_0
   \right)
   \right|
   %%%% 1 %%%%
   \\
   & 
   \ 
   \le
   \ 
   \left| 
   1 / \pi_i
   -
   (
      f ^ { ' }
   )
   ^ {-1}
   \left( 
   \inner
   { B(X_i)}
   { \lambda ^ * }
   +
   \lambda^\dagger_0
   \right)
   \right|
      %%%% 1 a %%%%
   \\
   &
   \qquad
   +
   \ 
\left| 
   (
      f ^ { ' }
   )
   ^ {-1}
   \left( 
   \inner
   { B(X_i)}
   { \lambda ^ \dagger }
   +
   \lambda^\dagger_0
   \right)
   -
   (
      f ^ { ' }
   )
   ^ {-1}
   \left( 
   \inner
   { B(X_i)}
   { \lambda ^ *}
   +
   \lambda^\dagger_0
   \right)
   \right|
      %%%% 2 %%%%
   \\
   &
   \ 
   =:
   I_1 +
   I_2
 \end{align*}
 By the universal consistency of $B$ and the continuity of $(f^{'})^{-1}$ the first term converges to $0$ in probability.
 By the continuity of $(f^{'})^{-1}$,
 the uniform boundedness of $\norm{B}$ and the dual consistency
 the second term converges to $0$ in probability.

